otbn_model/dafny_library/NativeTypes.dfy
@@ -1,0 +1,31 @@
+module NativeTypes {
+  const BASE_0:   int := 1
+
+  const BASE_1:   int := 2
+  const BASE_2:   int := 4
+  const BASE_4:   int := 16
+  const BASE_5:   int := 32
+  const BASE_8:   int := 0x1_00
+  const BASE_16:  int := 0x1_0000
+  const BASE_24:  int := 0x1_000000
+  const BASE_32:  int := 0x1_00000000
+  const BASE_40:  int := 0x1_00000000_00
+  const BASE_48:  int := 0x1_00000000_0000
+  const BASE_56:  int := 0x1_00000000_000000
+  const BASE_64:  int := 0x1_00000000_00000000
+  const BASE_128: int := 0x1_00000000_00000000_00000000_00000000
+  const BASE_256: int := 0x1_00000000_00000000_00000000_00000000_00000000_00000000_00000000_00000000
+  const BASE_512: int :=
+  0x1_00000000_00000000_00000000_00000000_00000000_00000000_00000000_00000000_00000000_00000000_00000000_00000000_00000000_00000000_00000000_00000000;
+
+  newtype {:nativeType "byte"} uint8 = x: int | 0 <= x < BASE_8
+  newtype uint16 = x: int | 0 <= x < BASE_16
+  newtype uint32 = x: int | 0 <= x < BASE_32
+  newtype uint64 = x: int | 0 <= x < BASE_64
+
+  newtype {:nativeType "sbyte"} int8 = x: int | -0x80 <= x < 0x80
+  newtype {:nativeType "short"} int16 = x: int | -0x8000 <= x < 0x8000
+  newtype {:nativeType "int"} int32 = x: int | -0x8000_0000 <= x < 0x8000_0000
+  newtype {:nativeType "long"} int64 = x: int | -0x8000_0000_0000_0000 <= x < 0x8000_0000_0000_0000
+
+}
