otbn_model/dafny_library/Sequences/NatSeq.dfy
@@ -1,0 +1,597 @@
+include "../Nonlinear_Arithmetic/DivMod.dfy"
+include "../Nonlinear_Arithmetic/Mul.dfy"
+include "../Nonlinear_Arithmetic/Power.dfy"
+include "Seq.dfy"
+
+abstract module NatSeq {
+
+  import opened DivMod
+  import opened Mul
+  import opened Power
+  import opened Seq
+
+  function method BASE(): nat
+		ensures BASE() > 1
+  type uint = i: int | 0 <= i < BASE()
+
+  //////////////////////////////////////////////////////////////////////////////
+  //
+  // to_nat definition and lemmas
+  //
+  //////////////////////////////////////////////////////////////////////////////
+
+  /* Converts a sequence to nat beginning from the lsw. */
+  function method {:opaque} to_nat(xs: seq<uint>): nat
+  {
+    if |xs| == 0 then 0
+    else
+      lemma_mul_nonnegative_auto();
+      to_nat(drop_first(xs)) * BASE() + first(xs)
+  }
+
+  /* Converts a sequence to nat beginning from the msw. */
+  function method {:opaque} to_nat_rev(xs: seq<uint>): nat
+  {
+    if |xs| == 0 then 0
+    else
+      lemma_power_positive_auto();
+      lemma_mul_nonnegative_auto();
+      to_nat_rev(drop_last(xs)) + last(xs) * power(BASE(), |xs| - 1)
+  }
+
+  /* Given the same sequence, to_nat and to_nat_rev return the same value. */
+  lemma lemma_to_nat_eq_to_nat_rev(xs: seq<uint>)
+    ensures to_nat(xs) == to_nat_rev(xs)
+  {
+    reveal to_nat();
+    reveal to_nat_rev();
+    if xs != [] {
+      if drop_last(xs) == [] {
+        calc {
+          to_nat_rev(xs);
+          last(xs) * power(BASE(), |xs| - 1);
+          { lemma_power_0_auto(); }
+          to_nat(xs);
+        }
+      } else {
+        calc {
+          to_nat_rev(xs);
+          to_nat_rev(drop_last(xs)) + last(xs) * power(BASE(), |xs| - 1);
+          { lemma_to_nat_eq_to_nat_rev(drop_last(xs)); }
+          to_nat(drop_last(xs)) + last(xs) * power(BASE(), |xs| - 1);
+          to_nat(drop_first(drop_last(xs))) * BASE() + first(xs) + last(xs)
+            * power(BASE(), |xs| - 1);
+          { lemma_to_nat_eq_to_nat_rev(drop_first(drop_last(xs))); }
+          to_nat_rev(drop_first(drop_last(xs))) * BASE() + first(xs) + last(xs)
+            * power(BASE(), |xs| - 1);
+          {
+            assert drop_first(drop_last(xs)) == drop_last(drop_first(xs));
+            reveal power();
+            lemma_mul_properties();
+          }
+          to_nat_rev(drop_last(drop_first(xs))) * BASE() + first(xs) + last(xs)
+            * power(BASE(), |xs| - 2) * BASE();
+          { lemma_mul_is_distributive_add_other_way_auto(); }
+          to_nat_rev(drop_first(xs)) * BASE() + first(xs);
+          { lemma_to_nat_eq_to_nat_rev(drop_first(xs)); }
+          to_nat(xs);
+        }
+      }
+    }
+  }
+
+  lemma lemma_to_nat_eq_to_nat_rev_auto()
+    ensures forall xs: seq<uint> {:trigger to_nat_rev(xs)}{:trigger to_nat(xs)}
+      :: to_nat(xs) == to_nat_rev(xs)
+  {
+    reveal to_nat();
+    reveal to_nat_rev();
+    forall xs: seq<uint> {:trigger to_nat_rev(xs)}{:trigger to_nat(xs)}
+      ensures to_nat(xs) == to_nat_rev(xs)
+    {
+      lemma_to_nat_eq_to_nat_rev(xs);
+    }
+  }
+
+  /* Proves the nat representation of a sequence of length 1. */
+  lemma lemma_seq_len_1(xs: seq<uint>)
+    requires |xs| == 1
+    ensures to_nat(xs) == first(xs)
+  {
+    reveal to_nat();
+  }
+
+  /* Proves the nat representation of a sequence of length 2. */
+  lemma lemma_seq_len_2(xs: seq<uint>)
+    requires |xs| == 2
+    ensures to_nat(xs) == first(xs) + xs[1] * BASE()
+  {
+    reveal to_nat();
+    lemma_seq_len_1(drop_last(xs));
+  }
+
+  /* Proves the nat representation of a sequence is bounded by BASE() to the
+  power of the sequence length. */
+  lemma lemma_seq_nat_bound(xs: seq<uint>)
+    ensures to_nat(xs) == to_nat_rev(xs) < power(BASE(), |xs|)
+  {
+    reveal to_nat_rev();
+    lemma_to_nat_eq_to_nat_rev_auto();
+    reveal power();
+    if |xs| != 0 {
+      var len' := |xs| - 1;
+      var pow := power(BASE(), len');
+      calc {
+        to_nat(xs);
+        to_nat_rev(xs);
+        to_nat_rev(drop_last(xs)) + last(xs) * pow;
+        <  { lemma_seq_nat_bound(drop_last(xs)); }
+        pow + last(xs) * pow;
+        <= {
+            lemma_power_positive_auto();
+            lemma_mul_inequality_auto();
+           }
+        pow + (BASE() - 1) * pow;
+           { lemma_mul_is_distributive_auto(); }
+        power(BASE(), len' + 1);
+      }
+    }
+  }
+
+  /* Nat representation of a sequence based on its prefix. */
+  lemma lemma_seq_prefix(xs: seq<uint>, i: nat)
+    requires 0 <= i <= |xs|
+    ensures to_nat(xs[..i]) + to_nat(xs[i..]) * power(BASE(), i) == to_nat(xs)
+  {
+    reveal to_nat();
+    reveal power();
+    if i == 1 {
+      assert to_nat(xs[..1]) == first(xs);
+    } else if i > 1 {
+      calc {
+        to_nat(xs[..i]) + to_nat(xs[i..]) * power(BASE(), i);
+        to_nat(drop_first(xs[..i])) * BASE() + first(xs) + to_nat(xs[i..]) * power(BASE(), i);
+          {
+            assert drop_first(xs[..i]) == drop_first(xs)[..i-1];
+            lemma_mul_properties();
+          }
+        to_nat(drop_first(xs)[..i-1]) * BASE() + first(xs) + (to_nat(xs[i..]) * power(BASE(), i - 1)) * BASE();
+          { lemma_mul_is_distributive_add_other_way_auto(); }
+        (to_nat(drop_first(xs)[..i-1]) + to_nat(drop_first(xs)[i-1..]) * power(BASE(), i - 1)) * BASE() + first(xs);
+          { lemma_seq_prefix(drop_first(xs), i - 1); }
+        to_nat(xs);
+      }
+    }
+  }
+
+  /* If there is an inequality between the most signficant words of two
+  sequences, then there is an inequality between the nat representations of
+  those sequences. */
+  lemma lemma_seq_msw_inequality(xs: seq<uint>, ys: seq<uint>)
+    requires |xs| == |ys| > 0
+    requires last(xs) < last(ys)
+    ensures to_nat(xs) < to_nat(ys)
+  {
+    reveal to_nat_rev();
+    lemma_to_nat_eq_to_nat_rev_auto();
+    var len' := |xs| - 1;
+    calc {
+      to_nat(xs);
+      to_nat_rev(xs);
+      <  { lemma_seq_nat_bound(drop_last(xs)); }
+      power(BASE(), len') + last(xs) * power(BASE(), len');
+      == { lemma_mul_is_distributive_auto(); }
+      (1 + last(xs)) * power(BASE(), len');
+      <= { lemma_power_positive_auto(); lemma_mul_inequality_auto(); }
+      to_nat_rev(ys);
+      to_nat(ys);
+    }
+  }
+
+  /* If two sequence prefixes do not have the same nat representations, then the two sequences do not have the same nat representations. */
+  lemma lemma_seq_prefix_neq(xs: seq<uint>, ys: seq<uint>, i: nat)
+    requires 0 <= i <= |xs| == |ys|
+    requires to_nat(xs[..i]) != to_nat(ys[..i])
+    ensures to_nat(xs) != to_nat(ys)
+    decreases |xs| - i
+  {
+    if i == |xs| {
+      assert xs[..i] == xs;
+      assert ys[..i] == ys;
+    } else {
+      if xs[i] == ys[i] {
+        reveal to_nat_rev();
+        assert drop_last(xs[..i+1]) == xs[..i];
+        assert drop_last(ys[..i+1]) == ys[..i];
+
+        lemma_to_nat_eq_to_nat_rev_auto();
+        assert to_nat(xs[..i+1]) == to_nat_rev(xs[..i+1]);
+      } else {
+        if xs[i] < ys[i]  { lemma_seq_msw_inequality(xs[..i+1], ys[..i+1]); }
+        else              { lemma_seq_msw_inequality(ys[..i+1], xs[..i+1]); }
+      }
+      lemma_seq_prefix_neq(xs, ys, i + 1);
+    }
+  }
+
+  /* If two sequences are not equal, their nat representations are not equal. */
+  lemma lemma_seq_neq(xs: seq<uint>, ys: seq<uint>, n: nat)
+    requires |xs| == |ys| == n
+    requires xs != ys
+    ensures to_nat(xs) != to_nat(ys)
+  {
+    ghost var i: nat := 0;
+
+    while i < n
+      invariant 0 <= i < n
+      invariant xs[..i] == ys[..i]
+    {
+      if xs[i] != ys[i] {
+        break;
+      }
+      i := i + 1;
+    }
+    assert to_nat_rev(xs[..i]) == to_nat_rev(ys[..i]);
+
+    reveal to_nat_rev();
+    assert xs[..i+1][..i] == xs[..i];
+    assert ys[..i+1][..i] == ys[..i];
+    lemma_power_positive_auto();
+    lemma_mul_strict_inequality_auto();
+    assert to_nat_rev(xs[..i+1]) != to_nat_rev(ys[..i+1]);
+    lemma_to_nat_eq_to_nat_rev_auto();
+
+    lemma_seq_prefix_neq(xs, ys, i+1);
+  }
+
+  /* Proves mod equivalence between the nat representation of a sequence and
+  the lsw of the sequence.*/
+  lemma lemma_seq_lsw_mod_equivalence(xs: seq<uint>)
+    requires |xs| >= 1;
+    ensures is_mod_equivalent(to_nat(xs), first(xs), BASE());
+  {
+    if |xs| == 1 {
+      lemma_seq_len_1(xs);
+      lemma_mod_equivalence_auto();
+    } else {
+      assert is_mod_equivalent(to_nat(xs), first(xs), BASE()) by {
+        reveal to_nat();
+        calc ==> {
+          true;
+            { lemma_mod_equivalence_auto(); }
+          is_mod_equivalent(to_nat(xs),
+                            to_nat(drop_first(xs)) * BASE() + first(xs),
+                            BASE());
+            { lemma_mod_multiples_basic_auto(); }
+          is_mod_equivalent(to_nat(xs), first(xs), BASE());
+        }
+      }
+    }
+  }
+
+  //////////////////////////////////////////////////////////////////////////////
+  //
+  // to_seq definition and lemmas
+  //
+  //////////////////////////////////////////////////////////////////////////////
+
+  /* Converts a nat to a sequence. */
+  function method {:opaque} to_seq(n: nat): seq<uint>
+  {
+    if n == 0 then []
+    else
+      lemma_div_basics_auto();
+      lemma_div_decreases_auto();
+      [n % BASE()] + to_seq(n / BASE())
+  }
+
+  /* Converts a nat to a sequence of a specified length. */
+  function method {:opaque} to_seq_with_len(n: nat, len: nat): (xs: seq<uint>)
+    requires power(BASE(), len) > n
+    ensures |xs| == len
+  {
+    reveal power();
+    if n == 0 then
+      (if len == 0 then []
+       else
+        lemma_power_positive(BASE(), len - 1);
+        [0] + to_seq_with_len(n, len - 1))
+    else
+      lemma_div_basics_auto();
+      lemma_div_decreases_auto();
+      lemma_multiply_divide_lt_auto();
+      [n % BASE()] + to_seq_with_len(n / BASE(), len - 1)
+  }
+
+  /* nat representation of an all zero sequence is 0. */
+  lemma lemma_to_seq_with_len_zero(len: nat)
+    ensures power(BASE(), len) > 0
+    ensures to_nat(to_seq_with_len(0, len)) == 0
+  {
+    reveal to_nat();
+    reveal to_seq_with_len();
+    lemma_power_positive(BASE(), len);
+    if len > 0 {
+      calc {
+        to_nat(to_seq_with_len(0, len));
+        to_nat([0] + to_seq_with_len(0, len - 1));
+        to_nat(to_seq_with_len(0, len - 1)) * BASE();
+          {
+            lemma_to_seq_with_len_zero(len - 1);
+            lemma_mul_basics_auto();
+          }
+        0;
+      }
+    }
+  }
+
+  /* Proves that if we start with a nat, convert it to a sequence using to_seq
+  and to_seq_with_len, and convert it back, the resulting numbers are
+  equivalent. */
+  lemma lemma_to_seq_with_len_eq_to_seq(n: nat, len: nat)
+    requires power(BASE(), len) > n
+    ensures to_nat(to_seq_with_len(n, len)) == to_nat(to_seq(n))
+  {
+    reveal to_nat();
+    reveal to_seq_with_len();
+    reveal to_seq();
+    if n == 0 && len != 0 {
+      lemma_to_seq_with_len_zero(len);
+    } else if n > 0 {
+      calc {
+        to_nat(to_seq_with_len(n, len));
+          {
+            lemma_div_basics_auto();
+            lemma_multiply_divide_lt_auto();
+          }
+        to_nat([n % BASE()] + to_seq_with_len(n / BASE(), len - 1));
+        to_nat([n % BASE()]) + to_nat(to_seq_with_len(n / BASE(), len - 1)) * BASE();
+          {
+            lemma_div_decreases_auto();
+            lemma_to_seq_with_len_eq_to_seq(n / BASE(), len - 1);
+          }
+        to_nat([n % BASE()]) + to_nat(to_seq(n / BASE())) * BASE();
+        to_nat(to_seq(n));
+      }
+    }
+  }
+
+  /* Proves that if we start with a nat, convert it to a sequence, and convert
+  it back, we get the same nat we started with. */
+  lemma lemma_nat_seq_nat(n: nat)
+    ensures to_nat(to_seq(n)) == n
+    decreases n
+  {
+    reveal to_nat();
+    reveal to_seq();
+    if n > 0 {
+      calc {
+        to_nat(to_seq(n));
+          { lemma_div_basics_auto(); }
+        to_nat([n % BASE()] + to_seq(n / BASE()));
+        n % BASE() + to_nat(to_seq(n / BASE())) * BASE();
+          {
+            lemma_div_decreases_auto();
+            lemma_nat_seq_nat(n / BASE());
+          }
+        n % BASE() + n / BASE() * BASE();
+          { lemma_fundamental_div_mod(n, BASE()); }
+        n;
+      }
+    }
+  }
+
+  //////////////////////////////////////////////////////////////////////////////
+  //
+  // Sequences with zeros
+  //
+  //////////////////////////////////////////////////////////////////////////////
+
+  /* Generates a sequence of zeros with length len. */
+  function method {:opaque} seq_zero(len: nat): (zs: seq<uint>)
+    ensures |zs| == len
+  {
+    if len == 0 then [] else [0] + seq_zero(len - 1)
+  }
+
+  /* nat representation of an all zero sequence is 0. */
+  lemma lemma_seq_zero_nat(len: nat)
+    ensures to_nat(seq_zero(len)) == 0
+  {
+    reveal to_nat();
+    if len > 0 {
+      calc {
+        to_nat(seq_zero(len));
+          { reveal seq_zero(); }
+        to_nat([0] + seq_zero(len - 1));
+        to_nat(seq_zero(len - 1)) * BASE() + 0;
+          {
+            lemma_seq_zero_nat(len - 1);
+            lemma_mul_basics_auto();
+          }
+        0;
+      }
+    }
+  }
+
+  /* Prepending a zero is equal to multiplying the nat representation of the
+  sequence by BASE(). */
+  lemma lemma_seq_prepend_zero(xs: seq<uint>)
+    ensures to_nat([0] + xs) == to_nat(xs) * BASE()
+  {
+    reveal to_nat();
+  }
+
+  /* Appending a zero does not change the nat representation of the sequence. */
+  lemma lemma_seq_append_zero(xs: seq<uint>) 
+    ensures to_nat(xs + [0]) == to_nat(xs)
+  {
+    reveal to_nat_rev();
+    lemma_to_nat_eq_to_nat_rev_auto();
+    calc == {
+      to_nat(xs + [0]);
+      to_nat_rev(xs + [0]);
+      to_nat_rev(xs) + 0 * power(BASE(), |xs|);
+        { lemma_mul_basics_auto(); }
+      to_nat_rev(xs);
+      to_nat(xs);
+    }
+  }
+
+  /* Extend a sequence to a specified length. */
+  function method {:opaque} seq_extend(xs: seq<uint>, n: nat): (ys: seq<uint>)
+    requires |xs| <= n
+    ensures |ys| == n
+    decreases n - |xs|
+  {
+    if |xs| >= n then xs else seq_extend(xs + [0], n)
+  }
+
+  //////////////////////////////////////////////////////////////////////////////
+  //
+  // Addition and subtraction
+  //
+  //////////////////////////////////////////////////////////////////////////////
+
+  /* Adds two sequences. */
+  function method {:opaque} seq_add(xs: seq<uint>,
+                                    ys: seq<uint>): (seq<uint>, nat)
+    requires |xs| == |ys|
+    ensures var (zs, cout) := seq_add(xs, ys); |zs| == |xs|
+  {
+    reveal seq_add();
+    if |xs| == 0 then ([], 0)
+    else
+      var (zs', cin) := seq_add(drop_last(xs), drop_last(ys));
+      var sum: int := last(xs) + last(ys) + cin;
+      var (sum_out, cout) := if sum < BASE() then (sum, 0) else (sum - BASE(), 1);
+      (zs' + [sum_out], cout)
+  }
+
+  /* Proves seq_add yields the same value as converting the sequences to nats,
+  then adding them. */
+  lemma lemma_seq_add_nat(xs: seq<uint>,
+                          ys: seq<uint>,
+                          zs: seq<uint>,
+                          cout: nat)
+    requires |xs| == |ys|
+    requires seq_add(xs, ys) == (zs, cout)
+    ensures to_nat(xs) + to_nat(ys) == to_nat(zs) + cout * power(BASE(), |xs|)
+  {
+    reveal seq_add();
+    if |xs| == 0 {
+      reveal to_nat();
+    } else {
+      var pow := power(BASE(), |xs| - 1);
+      var (zs', cin) := seq_add(drop_last(xs), drop_last(ys));
+      var sum: int := last(xs) + last(ys) + cin;
+      var z := if sum < BASE() then sum else sum - BASE();
+      assert sum == z + cout * BASE();
+
+      reveal to_nat_rev();
+      lemma_to_nat_eq_to_nat_rev_auto();
+      calc {
+        to_nat(zs);
+        to_nat_rev(zs);
+        to_nat_rev(zs') + z * pow;
+          { lemma_seq_add_nat(drop_last(xs), drop_last(ys), zs', cin); }
+        to_nat_rev(drop_last(xs)) + to_nat_rev(drop_last(ys)) - cin * pow + z * pow;
+          {
+            lemma_mul_equality_auto();
+            assert sum * pow == (z + cout * BASE()) * pow;
+            lemma_mul_is_distributive_auto();
+          } 
+        to_nat_rev(xs) + to_nat_rev(ys) - cout * BASE() * pow;
+          {
+            lemma_mul_is_associative(cout, BASE(), pow);
+            reveal power();
+          }
+        to_nat_rev(xs) + to_nat_rev(ys) - cout * power(BASE(), |xs|);
+        to_nat(xs) + to_nat(ys) - cout * power(BASE(), |xs|);
+      }
+    }
+  }
+
+  /* Subtracts two sequences. */
+  function method {:opaque} seq_sub(xs: seq<uint>,
+                                    ys: seq<uint>): (seq<uint>, nat)
+    requires |xs| == |ys|
+    ensures var (zs, cout) := seq_sub(xs, ys); |zs| == |xs|
+  {
+    reveal seq_sub();
+    if |xs| == 0 then ([], 0)
+    else 
+      var (zs, cin) := seq_sub(drop_last(xs), drop_last(ys));
+      var (diff_out, cout) := if last(xs) >= last(ys) + cin
+                              then (last(xs) - last(ys) - cin, 0)
+                              else (BASE() + last(xs) - last(ys) - cin, 1);
+      (zs + [diff_out], cout)
+  }
+
+  /* Proves seq_sub yields the same value as converting the sequences to nats,
+  then subtracting them. */
+  lemma lemma_seq_sub_nat(xs: seq<uint>,
+                          ys: seq<uint>,
+                          zs: seq<uint>,
+                          cout: nat)
+    requires |xs| == |ys|
+    requires seq_sub(xs, ys) == (zs, cout)
+    ensures to_nat(xs) - to_nat(ys) + cout * power(BASE(), |xs|) == to_nat(zs)
+  {
+    reveal seq_sub();
+    if |xs| == 0 {
+      reveal to_nat();
+    } else {
+      var pow := power(BASE(), |xs| - 1);
+      var (zs', cin) := seq_sub(drop_last(xs), drop_last(ys));
+      var z := if last(xs) >= last(ys) + cin
+               then last(xs) - last(ys) - cin
+               else BASE() + last(xs) - last(ys) - cin;
+      assert cout * BASE() + last(xs) - cin - last(ys) == z;
+
+      reveal to_nat_rev();
+      lemma_to_nat_eq_to_nat_rev_auto();
+      calc {
+        to_nat(zs);
+        to_nat_rev(zs);
+        to_nat_rev(zs') + z * pow;
+          { lemma_seq_sub_nat(drop_last(xs), drop_last(ys), zs', cin); }
+        to_nat_rev(drop_last(xs)) - to_nat_rev(drop_last(ys)) + cin * pow + z * pow;
+          {
+            lemma_mul_equality_auto();
+            assert pow * (cout * BASE() + last(xs) - cin - last(ys)) == pow * z;
+            lemma_mul_is_distributive_auto();
+          }
+        to_nat_rev(xs) - to_nat_rev(ys) + cout * BASE() * pow;
+          {
+            lemma_mul_is_associative(cout, BASE(), pow);
+            reveal power();
+          }
+        to_nat_rev(xs) - to_nat_rev(ys) + cout * power(BASE(), |xs|);
+        to_nat(xs) - to_nat(ys) + cout * power(BASE(), |xs|);
+      }
+    }
+  }
+
+}
+
+abstract module NatSeq1 refines NatSeq {
+
+  function method BASE1(): nat
+		ensures BASE1() > 1
+
+  function method BASE(): nat { BASE1() }
+
+}
+
+abstract module NatSeq2 refines NatSeq {
+
+  import NatSeq1
+
+  function method BASE2(): nat
+		ensures BASE2() > 1
+      && exists n :: (NatSeq1.BASE() == power(BASE2(), n) && n > 1)
+
+  function method BASE(): nat { BASE2() }
+
+}
