otbn_model/dafny_library/Sequences/NatSeqConversions.dfy
@@ -1,0 +1,58 @@
+include "NatSeq.dfy"
+
+abstract module NatSeqConversions refines NatSeq {
+
+  import NatSeq1
+  import NatSeq2
+
+  function N(): nat
+  {
+    var n: nat :| NatSeq1.BASE() == power(NatSeq2.BASE(), n) && n > 1;
+    n
+  }
+
+  function {:opaque} to_lower_base(xs: seq<NatSeq1.uint>): seq<NatSeq2.uint>
+  {
+    if xs == [] then []
+    else NatSeq2.to_seq_with_len(first(xs), N()) + to_lower_base(drop_first(xs))
+  }
+
+  function {:opaque} to_higher_base(xs: seq<NatSeq2.uint>): seq<NatSeq1.uint>
+  {
+    if xs == [] then []
+    else
+      if |xs| < N() then
+        NatSeq2.lemma_seq_nat_bound(xs);
+        lemma_power_strictly_increases(NatSeq2.BASE(), |xs|, N());
+        [NatSeq2.to_nat(xs) as NatSeq1.uint]
+      else
+        NatSeq2.lemma_seq_nat_bound(xs[..N()]);
+        lemma_mod_sub_multiples_vanish_auto();
+        [NatSeq2.to_nat(xs[..N()]) as NatSeq1.uint] + to_higher_base(xs[N()..])
+  }
+
+  lemma lemma_to_lower_base(xs: seq<NatSeq1.uint>)
+    ensures NatSeq2.to_nat(to_lower_base(xs)) == NatSeq1.to_nat(xs)
+  {
+    reveal NatSeq1.to_nat();
+    reveal NatSeq2.to_nat();
+    reveal to_lower_base();
+    if xs != [] {
+      calc {
+        NatSeq2.to_nat(to_lower_base(xs));
+        NatSeq2.to_nat(NatSeq2.to_seq_with_len(first(xs), N()) + to_lower_base(drop_first(xs)));
+          { NatSeq2.lemma_seq_prefix(NatSeq2.to_seq_with_len(first(xs), N()) + to_lower_base(drop_first(xs)), N()); }
+        NatSeq2.to_nat(NatSeq2.to_seq_with_len(first(xs), N())) + NatSeq2.to_nat(to_lower_base(drop_first(xs))) * power(NatSeq2.BASE(), N());
+          {
+            NatSeq2.lemma_to_seq_with_len_eq_to_seq(first(xs), N());
+            NatSeq2.lemma_nat_seq_nat(first(xs));
+            lemma_to_lower_base(drop_first(xs));
+          }
+        first(xs) + NatSeq1.to_nat(drop_first(xs)) * power(NatSeq2.BASE(), N());
+          { assert power(NatSeq2.BASE(), N()) == NatSeq1.BASE(); }
+        NatSeq1.to_nat(xs);
+      }
+    }
+  }
+
+}
